proof/correctness/Correctness_Hash.ec
@@ -3,34 +3,112 @@ pragma Goals : printall.
 require import AllCore List RealExp IntDiv.
 from Jasmin require import JModel.
 
-require import RandomBytes XMSS_IMPL XMSS_IMPL_HOP1.
-require import Address Notation Primitives XMSS_MT_PRF.
+require import RandomBytes XMSS_IMPL.
+require import Address Notation Hash Primitives Params Parameters Utils Util.
+require import Correctness_Mem.
 
-require import Array8 Array32 Array64 Array128.
+require import Array8 Array32 Array64 Array96 Array128.
 (*---*) import NBytes.
 
-require import Utils. (* valid_ptr *)
+axiom hash_96 (x : W8.t Array96.t) :
+    phoare[M(Syscall).__core_hash_96 : arg.`2 = x ==> to_list res = Hash (to_list x)] = 1%r.
 
-pred array32_list_eq (x : W8.t Array32.t) (y : W8.t list) = 
-  forall (k : int), 0 <= k < 32 => x.[k] = nth witness y k.
+axiom hash_128 (x : W8.t Array128.t) :
+    phoare[M(Syscall).__core_hash_128 : arg.`2 = x ==> to_list res = Hash (to_list x)] = 1%r.
 
-axiom hash_ptr (mem : global_mem_t) (ptr inlen : W64.t) :
-  array32_list_eq (Hash_ptr ptr inlen) (Hash (mkseq (fun (i : int) => loadW8 mem ((W64.to_uint ptr) + i)) (to_uint inlen))).
+lemma prf_correctness (a b : W8.t Array32.t) :
+    prf_padding_val = XMSS_HASH_PADDING_PRF /\ 
+    padding_len = XMSS_PADDING_LEN =>
+    equiv [
+    M(Syscall).__prf ~ Hash.prf : 
+    arg{1}.`2 = a /\ arg{1}.`3 = b /\ arg{2} = (to_list a, to_list b) 
+    ==>
+    res{2} = to_list res{1}
+    ].
+proof.
+rewrite /XMSS_HASH_PADDING_PRF /XMSS_PADDING_LEN => [#] ??.
+proc.
+seq 9 2 : (buf{2} = to_list buf{1}); last first.
+  + inline M(Syscall).__core_hash__96 M(Syscall)._core_hash_96; wp; sp.
+    ecall {1} (hash_96 buf{1}); auto => /> /#.
+seq 3 0 : (#pre); 1:auto.
+seq 1 1 : (#pre /\ padding{2} = to_list padding_buf{1}).
+  + call {1} (ull_to_bytes_correct (of_int 3)%W64); auto => />. 
+seq 1 0 : (
+  key{2} = to_list key{1} /\
+  in_0{2} = to_list in_0{1} /\
+  padding{2} = to_list padding_buf{1} /\ 
+  forall (k : int), 0 <= k < 32 => buf{1}.[k] = nth witness padding{2} k
+); first by auto => /> *; smt(@Array96 @List).
+seq 1 0 : (#pre /\ aux{1} = key{1}); first by ecall {1} (_x_memcpy_u8u8_post key{1}); auto => />.
+seq 1 0 : (#pre /\ forall (k : int), 32 <= k < 64 => buf{1}.[k] = nth witness key{2} (k - 32)).
+    + auto => />; smt(@Array96 @List).
+seq 1 0 : (
+  key{2} = to_list key{1} /\
+  in_0{2} = to_list in_0{1} /\
+  padding{2} = to_list padding_buf{1} /\ 
+  (forall (k : int), 0 <= k < 32 => buf{1}.[k] = nth witness padding{2} k) /\
+  (forall (k : int), 32 <= k < 64 => buf{1}.[k] = nth witness key{2} (k - 32)) /\
+  aux{1} = in_0{1}
+).
+    + ecall {1} (_x_memcpy_u8u8_post in_0{1}); auto => /> /#.
+seq 1 0 : (
+  key{2} = to_list key{1} /\ size key{2} = 32 /\
+  in_0{2} = to_list in_0{1} /\ size in_0{2} = 32 /\
+  padding{2} = to_list padding_buf{1} /\  size padding{2} = 32 /\
+  (forall (k : int), 0 <= k < 32 => buf{1}.[k] = nth witness padding{2} k) /\
+  (forall (k : int), 32 <= k < 64 => buf{1}.[k] = nth witness key{2} (k - 32)) /\
+  (forall (k : int), 64 <= k < 96 => buf{1}.[k] = nth witness in_0{2} (k - 64))
+).
+    + auto => /> *; do split; smt(@Array96 @List).
+    + auto => /> *; rewrite !/to_list !/mkseq -!iotaredE => /> /#. 
+qed.
 
-op addr_to_bytes (a : W32.t Array8.t) : W8.t Array32.t.
-
-(* PRF *)
-(* Spec: op PRF : seed -> adrs -> key. *)
-(* IMPL: op _PRF_ : W8.t Array32.t -> W8.t Array32.t -> W8.t Array32.t -> W8.t Array32.t. *)
-op _PRF_ : W8.t Array32.t -> W8.t Array32.t -> W8.t Array32.t -> W8.t Array32.t.
-
-axiom prf_equiv (out : W8.t Array32.t, addr : W32.t Array8.t, seed : W8.t Array32.t) :
-  PRF (to_list seed) addr = to_list (_PRF_ out (addr_to_bytes addr) seed).
-
-
-(* spec: op F : key -> nbytes -> nbytes. *)
-(* impl: op Hash : W8.t list -> W8.t list.*)
-axiom hash_F_equiv (a : key, b : nbytes) : F a b = Hash (a ++ b).
-
-
-search Array64.init.
+lemma prf_keygen_correctness (a : W8.t Array64.t, b : W8.t Array32.t) :
+    prf_padding_val = XMSS_HASH_PADDING_PRF /\
+    prf_kg_padding_val = XMSS_HASH_PADDING_PRF_KEYGEN /\ 
+    padding_len = XMSS_PADDING_LEN =>
+    equiv [
+    M(Syscall).__prf_keygen ~ Hash.prf_keygen : 
+    arg{1}.`2 = a /\ arg{1}.`3 = b /\ arg{2} = (to_list a, to_list b) 
+    ==>
+    res{2} = to_list res{1}
+    ].
+proof.
+rewrite /XMSS_HASH_PADDING_PRF_KEYGEN /XMSS_PADDING_LEN => [#] ???.
+proc => //=.
+seq 9 2 : (buf{2} = to_list buf{1}); last first.
+  + inline M(Syscall).__core_hash__128 M(Syscall)._core_hash_128; wp; sp.
+    ecall {1} (hash_128 buf{1}); auto => /> /#.
+seq 3 0 : (#pre); 1:auto.
+seq 1 1 : (#pre /\ padding{2} = to_list padding_buf{1}).
+  + call {1} (ull_to_bytes_correct (of_int 4)%W64); auto => />. 
+seq 1 0 : (
+  key{2} = to_list key{1} /\
+  in_0{2} = to_list in_0{1} /\
+  padding{2} = to_list padding_buf{1} /\ 
+  forall (k : int), 0 <= k < 32 => buf{1}.[k] = nth witness padding{2} k
+); first by auto => /> *; smt(@Array128 @List).
+seq 1 0 : (#pre /\ aux{1} = key{1}); first by ecall {1} (_x_memcpy_u8u8_post key{1}); auto => />.
+seq 1 0 : (#pre /\ forall (k : int), 32 <= k < 64 => buf{1}.[k] = nth witness key{2} (k - 32)).
+    + auto => />; smt(@Array128 @List).
+seq 1 0 : (
+  key{2} = to_list key{1} /\
+  in_0{2} = to_list in_0{1} /\
+  padding{2} = to_list padding_buf{1} /\ 
+  (forall (k : int), 0 <= k < 32 => buf{1}.[k] = nth witness padding{2} k) /\
+  (forall (k : int), 32 <= k < 64 => buf{1}.[k] = nth witness key{2} (k - 32)) /\
+  aux_0{1} = in_0{1}
+).
+    + ecall {1} (_x_memcpy_u8u8_64_post in_0{1}); auto => /> /#.
+seq 1 0 : (
+  key{2} = to_list key{1} /\ size key{2} = 32 /\
+  in_0{2} = to_list in_0{1} /\ size in_0{2} = 64 /\
+  padding{2} = to_list padding_buf{1} /\  size padding{2} = 32 /\
+  (forall (k : int), 0 <= k < 32 => buf{1}.[k] = nth witness padding{2} k) /\
+  (forall (k : int), 32 <= k < 64 => buf{1}.[k] = nth witness key{2} (k - 32)) /\
+  (forall (k : int), 64 <= k < 128 => buf{1}.[k] = nth witness in_0{2} (k - 64))
+).
+    + auto => /> *; do split; smt(@Array128 @List).
+    + auto => /> *; rewrite !/to_list !/mkseq -!iotaredE => /> /#. 
+qed.
