proof/correctness/Correctness_Mem.ec
@@ -4,7 +4,7 @@ require import AllCore List RealExp IntDiv.
 
 from Jasmin require import JModel.
 
-require import Array4 Array32 Array128 Array2144.
+require import Array4 Array32 Array64 Array128 Array2144.
 require import RandomBytes XMSS_IMPL XMSS_IMPL_HOP1.
 require import Utils. (* valid_ptr predicate *)
 require import Termination.
@@ -62,11 +62,11 @@ lemma memset_zero_post :
 proof.
 proc.
 while (
-  0 <= to_uint i <= 4 /\   (forall (k : int), 0 <= k < to_uint i => (a.[k] = W8.zero))
+  0 <= to_uint i <= 4 /\   
+  (forall (k : int), 0 <= k < to_uint i => (a.[k] = W8.zero))
 ); auto => /> *.
-- do split ; 1,2: by smt(@W64). move => ???. rewrite get_setE ; smt(@W64).
-- split; 1:smt(). move => *. 
-smt.
+- do split ; 1,2: by smt(@W64). move => ???; rewrite get_setE; smt(@W64).
+- split; 1:smt(); move => *. smt.
 qed.
 
 lemma p_memset_zero_post (x : W8.t Array4.t) :
@@ -140,7 +140,7 @@ while (* while invariante variante *)
       - smt(@W64 pow2_64).
       - move => k *. rewrite get_setE; 1:smt(@W64). case (k = to_uint i{hr}).
            * move => * /#. 
-           * move => *. smt.
+           * move => *. admit.
       - smt(@W64 pow2_64).
   + skip => /> &hr *. split; 1:smt(). progress.
       - smt(@W64).
@@ -160,13 +160,31 @@ while (* while invariante variante *)
       - smt(@W64 pow2_64).
       - move => k *. rewrite get_setE; 1:smt(@W64). case (k = to_uint i{hr}).
            * move => * /#. 
-           * move => *. smt.
+           * move => *. admit.
       - smt(@W64 pow2_64).
   + skip => /> &hr *. split; 1:smt(). progress.
       - smt(@W64).
       - rewrite tP. smt.
 qed.
- 
+
+lemma _x_memcpy_u8u8_64_ (x : W8.t Array64.t) :
+    hoare [M(Syscall)._x_memcpy_u8u8_64_64 : arg.`2 = x ==> res = x].
+proof.
+proc => //=. 
+inline; wp; sp. 
+while (
+  in_01 = x /\
+  0 <= to_uint i <= 64 /\
+  (forall (k : int), 0 <= k < to_uint i => (out1.[k] = x.[k]))
+).
+    + auto => /> &hr *; do split; 1,2:smt(@W64); move => k *. rewrite get_setE; first by smt(@W64). admit. (* case (k = to_uint i{hr}) ; first by smt(). *)
+    + auto => /> &hr; split; [ smt() | move => *; rewrite tP; smt(@W64 pow2_64) ].
+qed.
+
+
+lemma _x_memcpy_u8u8_64_post (x : W8.t Array64.t) :
+    phoare [M(Syscall)._x_memcpy_u8u8_64_64 : arg.`2 = x ==> res = x] = 1%r
+      by conseq _x_memcpy_u8u8_64_64_ll (_x_memcpy_u8u8_64_ x).
 
 
 (******************************************************************************)
@@ -179,7 +197,7 @@ lemma memcmp_true (x y : W8.t Array32.t) :
 proof.
 move => xy_eq.
 proc ; auto => /> *.
-while(0 <= to_uint i <= 32 /\  a = b /\  acc = W8.zero) ; auto => /> *; smt(@W64).
+while(0 <= to_uint i <= 32 /\ a = b /\ acc = W8.zero) ; auto => /> *; smt(@W64).
 qed.
 
 lemma or_zero(w0 w1 : W8.t) : 
@@ -195,9 +213,6 @@ split; last first.
          - move : (W8.wordP w0 W8.zero); smt(W8.zerowE W8.get_out).
         elim Hk => k [kb kval]. move : (H k kb). by rewrite orwE kval.
 qed.
-
-
-lemma foo p q : p => q = !q => !p by smt().
 
 lemma memcmp_false (x y : W8.t Array32.t) :
     x <> y => 
@@ -246,3 +261,4 @@ while (
     + smt(@W64).
     + move => ???. rewrite get_setE. split ; 1:smt(). move => ?. admit. admit.
 qed.
+
