proof/correctness/Utils.ec
@@ -6,31 +6,12 @@ require import BitEncoding.
 
 from Jasmin require import JModel.
 
-require import RandomBytes XMSS_IMPL XMSS_IMPL_HOP1.
+require import RandomBytes XMSS_IMPL Util.
 
 require import Array8 Array32.
 
-require import Params Parameters Address Notation Primitives Wots.
+require import Params Parameters Address Notation Primitives.
 (*---*) import NBytes.
-
-lemma size_nbytes (x : nbytes) : size x = n.
-proof.
-admit.
-qed.
-
-lemma size_wots_sk (sk : wots_sk) : size sk = len.
-proof.
-admit.
-qed.
-
-
-lemma size_flatten_wots_sk (sk : wots_sk) : size (flatten sk) = len * n.
-proof.
-rewrite size_flatten.
-admit.
-qed.
-
-(*** ***)
 
 pred valid_ptr (p o : W64.t) = 
   0 <= to_uint o => 
@@ -44,6 +25,15 @@ op addr_to_bytes (a : W32.t Array8.t) : W8.t list =
   let addr_bits : bool list = flatten (mkseq (fun (i : int) => W32.w2bits a.[i]) 8) in
   BitsToBytes addr_bits.
 
+(** -------------------------------------------------------------------------------------------- **)
+
+lemma ull_to_bytes_correct (x : W64.t) : 
+    equiv [M(Syscall).__ull_to_bytes_32 ~ Util.w64_to_bytes :
+      arg{1}.`2 = x /\ arg{2} = (x, 32)  ==> res{2} = to_list res{1}].
+proof.
+proc.
+admit.
+qed.
 
 lemma addr_to_bytes_correctness (x : W32.t Array8.t) : 
     phoare[M(Syscall).__addr_to_bytes : arg.`2 = x ==> to_list res = addr_to_bytes x] = 1%r.
@@ -59,42 +49,3 @@ proof.
 proc; inline.
 while (true) (8 - i); auto => /> /#.
 qed.
-
-(*
-lemma addr_to_bytes_correctness (x : W32.t Array8.t) : 
-    phoare[M_Hop1(Syscall).__addr_to_bytes :
-      arg.`2 = x ==> res = Array32.of_list witness (addr_to_bytes x)] = 1%r.
-proof.
-conseq (addr_to_bytes_ll) (addr_to_bytes_correctness x).
-auto => />.
-qed.
-*)
-
-lemma addr_to_bytes_hop1 :
-    equiv [M(Syscall).__addr_to_bytes ~ M_Hop1(Syscall).__addr_to_bytes : ={arg} ==> ={res}].  
-proof. proc ; sim => />. qed.
-
-(*** Hop 1 ***)
-
-lemma addr_to_bytes_hop1_ll : phoare [ M_Hop1(Syscall).__addr_to_bytes : true ==> true] = 1%r.
-proof.
-proc ; inline.
-while (true) (8 - i); auto => /> /#.
-qed.
-
-lemma addr_to_bytes_hop1_correctness (x : W32.t Array8.t) : 
-    hoare[M_Hop1(Syscall).__addr_to_bytes : arg.`2 = x ==> to_list res = addr_to_bytes x].
-proof.
-proc.
-auto => />. 
-admit.
-qed.
-
-lemma p_addr_to_bytes_hop1_correctness (x : W32.t Array8.t) : 
-    phoare[M_Hop1(Syscall).__addr_to_bytes :
-      arg.`2 = x ==> res = Array32.of_list witness (addr_to_bytes x)] = 1%r.
-proof.
-conseq (addr_to_bytes_hop1_ll) (addr_to_bytes_hop1_correctness x); auto => /> *.
-admit.
-qed.
-
